Azurite.lean
@@ -223,6 +223,10 @@ import Azurite.AzNat.Equiv.ModPow2
 import Azurite.AzNat.Equiv.Mul.Basic
 import Azurite.AzNat.Equiv.Mul.Karatsuba
 import Azurite.AzNat.Equiv.Mul.ToomCook3
+import Azurite.AzNat.Equiv.MulModPow2.Dispatch
+import Azurite.AzNat.Equiv.MulModPow2.Karatsuba
+import Azurite.AzNat.Equiv.MulModPow2.Schoolbook
+import Azurite.AzNat.Equiv.MulModPow2.ToomCook3
 import Azurite.AzNat.Equiv.NormalizedCompare
 import Azurite.AzNat.Equiv.OfLimbDigits
 import Azurite.AzNat.Equiv.OfLimbDigitsPow2
@@ -258,6 +262,10 @@ import Azurite.AzNat.Mul
 import Azurite.AzNat.Mul.Karatsuba
 import Azurite.AzNat.Mul.Schoolbook
 import Azurite.AzNat.Mul.ToomCook3
+import Azurite.AzNat.MulModPow2.Dispatch
+import Azurite.AzNat.MulModPow2.Karatsuba
+import Azurite.AzNat.MulModPow2.Schoolbook
+import Azurite.AzNat.MulModPow2.ToomCook3
 import Azurite.AzNat.NormalizedCompare
 import Azurite.AzNat.OfLimbDigits
 import Azurite.AzNat.OfLimbDigitsPow2
